Rewrite SIMT with Ssreflect.

SIMT.v
@@ -1,17 +1,23 @@
 Require Import SIMT_util.
-Require Import Vectors.VectorDef.
-Require Import ZArith.
-Import VectorNotations.
+Require Import ssreflect ssrfun ssrbool eqtype ssrnat seq fintype.
+Require Import tuple finfun finset ssrint intdiv.
 Require Import FunctionalExtensionality.
-Require Import ProofIrrelevance.
-Require Import Eqdep_dec.
-Require Import EqdepFacts.
+Open Scope list_scope.
+Import List.ListNotations.
 
 Section SIMT_Definition.
-  Variable num_threads : { n : nat & (n > 0)%nat}. (* the number of threads *)
-  Definition N := projT1 num_threads.
+  Local Notation "z < z'" := (intOrdered.ltz z z').
+  Local Notation "z <= z'" := (intOrdered.lez z z').
+  Local Notation "z + z'" := (intZmod.addz z z').
+  Local Notation "z * z'" := (intRing.mulz z z').
+  Implicit Arguments Vector_of_tuple [T n].
+  Implicit Arguments tuple_of_Vector [T n].
+
+  Variable num_threads : {n : nat | 0 < n}.
+  Definition N := sval num_threads.
 
   Definition arity := nat.
+  Definition arity_eqType := nat_eqType.
   Definition variable_name := nat.
 
   Inductive LV (n:arity) : Set :=
@@ -20,67 +26,164 @@ Section SIMT_Definition.
   Inductive SV (n:arity) : Set :=
   | shared : variable_name -> SV n.
 
-  Definition V n := (LV n + SV n)%type.
+  Inductive V n : Set :=
+  | local_variable : LV n -> V n
+  | shared_variable : SV n -> V n.
+  Coercion local_variable : LV >-> V.
+  Coercion shared_variable : SV >-> V.
 
-  Lemma eq_lv_dec : forall n (lv lv' : LV n), {lv = lv'} + {lv <> lv'}.
-    destruct n; destruct lv; destruct lv';
-    destruct (eq_nat_dec v v0) as [H | H];
-    try (subst; left; reflexivity);
-    try (right; contradict H; inversion H; reflexivity).
+  Definition eq_lv n (lv lv' : LV n) : bool :=
+    match lv, lv' with
+      | local l, local l' => l == l'
+    end.
+
+  Definition eq_sv n (sv sv' : SV n) : bool :=
+    match sv, sv' with
+      | shared l, shared l' => l == l'
+    end.
+
+  Definition eq_V n (v v' : V n) : bool :=
+    match v, v' with
+      | local_variable l, local_variable l' => eq_lv _ l l'
+      | shared_variable s, shared_variable s' => eq_sv _ s s'
+      | _, _ => false
+    end.
+
+  Lemma lv_eqP : forall n, Equality.axiom (eq_lv n).
+  Proof.
+    move => n.
+    case.
+    move => v y.
+    case: y => v'.
+    move H : (eq_lv _ _ _) => [];
+      rewrite/eq_lv in H; constructor; move: H;
+      repeat move/eqP => ?; congruence.
   Qed.
 
-  Lemma eq_sv_dec : forall n (sv sv' : SV n), {sv = sv'} + {sv <> sv'}.
-    destruct n; destruct sv; destruct sv';
-    destruct (eq_nat_dec v v0) as [H | H];
-    try (subst; left; reflexivity);
-    try (right; contradict H; inversion H; reflexivity).
+  Lemma sv_eqP : forall n, Equality.axiom (eq_sv n).
+    move => n.
+    case.
+    move => v y.
+    case: y => v'.
+    move H : (eq_sv _ _ _) => [];
+      rewrite/eq_lv in H; constructor; move: H;
+      repeat move/eqP => ?; congruence.
   Qed.
 
-  Definition Op n := t Z n -> Z.
+  Lemma V_eqP : forall n, Equality.axiom (eq_V n).
+  Proof.
+    move => n.
+    case.
+    { move => l y.
+      case: y => l'.
+      { rewrite /eq_V.
+        case: (lv_eqP n l l'); constructor; congruence. }
+      { constructor. done. }}
+    { move => s y.
+      case: y => s'.
+      { constructor. done. }
+      { rewrite /eq_V.
+        case: (sv_eqP n s s'); constructor; congruence. }
+    }
+  Qed.
 
-  Definition const (z:Z) : Op 0 := fun _ : t Z 0 => z.
+  Canonical lv_eqMixin n := EqMixin (lv_eqP n).
+  Canonical sv_eqMixin n := EqMixin (sv_eqP n).
+  Canonical lv_eqType n := Eval hnf in EqType _ (lv_eqMixin n).
+  Canonical sv_eqType n := Eval hnf in EqType _ (sv_eqMixin n).
+  Canonical V_eqMixin n := EqMixin (V_eqP n).
+  Canonical V_eqType n := Eval hnf in EqType _ (V_eqMixin n).
+
+
+  Definition Op n := n.-tuple int -> int.
+
+  Open Scope int_scope.
+  Definition const (z:int) : Op 0 := fun _ : 0.-tuple int => z.
   Definition e_plus : Op 2 :=
-    fun zs : t Z 2 => match zs return Z with
-                        | [x; y] => (x + y)%Z
-                        | _ => 0%Z
-                      end.
+    fun zs => match zs return int with
+                | Tuple [x; y] _ => x + y
+                | _ => 0
+              end.
+  Definition e_mult : Op 2 :=
+    fun zs => match zs return int with
+                | Tuple [x; y] _  => x * y
+                | _ => 0
+              end.
+  Definition e_div : Op 2 :=
+    fun zs => match zs with
+                | Tuple [x; y] _ => x %/ y
+                | _ => 0
+              end.
+  Definition int_of_bool := fun b => if b then 1%:Z else 0.
+  Definition bool_of_int := fun z : int => z != 0.
+  Lemma int_of_boolK : cancel int_of_bool bool_of_int.
+  Proof.
+    rewrite /cancel/int_of_bool/bool_of_int.
+    elim; done.
+  Qed.
   Definition e_neg : Op 1 :=
-    fun z : t Z 1 => match z return Z with
-                       | [0%Z] => 1%Z
-                       | _ => 0%Z
-                     end.
+    fun z => match z with
+               | Tuple [x] _ => int_of_bool (~~ (bool_of_int x))
+               | _ => 0
+             end.
   Definition e_and : Op 2 :=
-    fun zs : t Z 2 => match zs return Z with
-                        | [0%Z; y] => 0%Z
-                        | [x; 0%Z] => 0%Z
-                        | [x; y] => (Z.abs x + Z.abs y)%Z
-                        | _ => 0%Z
-                      end.
+    fun zs => match zs with
+                | Tuple [x; y] _ =>
+                  int_of_bool (andb (bool_of_int x)
+                                    (bool_of_int y))
+                | _ => 0
+              end.
   Definition e_lt : Op 2 :=
-    fun zs : t Z 2 => match zs return Z with
-                        | [x; y] => match (x ?= y)%Z with
-                                      | Lt => 1%Z
-                                      | _ => 0%Z
-                                    end
-                        | _ => 0%Z
-                      end.
+    fun zs => match zs with
+                | Tuple [x; y] _ =>
+                  int_of_bool (intOrdered.ltz x y)
+                | _ => 0
+              end.
+
+  Definition zero_tuple := tuple_of 0.
+  Record hoge : Type := { foo (A : Set) (B : Set) : A * B }.
 
   Inductive E : Set :=
   | tid : E
   | ntid : E
-  | var : forall n, V n -> t E n -> E
-  | func : forall n, Op n -> t E n -> E.
+  | var : forall n, V n -> Vector.t E n -> E
+  | func : forall n, Op n -> Vector.t E n -> E.
   Implicit Arguments var [n].
   Implicit Arguments func [n].
 
-  Notation "a '+' b" := (@func 2 e_plus [a; b]).
-  Notation "a '&&' b" := (@func 2 e_and [a; b]).
-  Notation "a '<' b" := (@func 2 e_lt [a; b]).
+  Lemma eqType_eq_rect_eq : forall (U : eqType) P (p : U) (x : P p) (H : p = p),
+                       x = eq_rect p P x p H.
+  Proof.
+    move=> U P p x H.
+      by rewrite (eq_irrelevance H erefl).
+  Qed.
+
+  Lemma eqType_eq_dep_eq :
+    forall (U : eqType) P (p : U) (x y : P p),
+      EqdepFacts.eq_dep U P p x p y -> x = y.
+  Proof.
+    move => U P p x y H.
+    case: (EqdepFacts.eq_dep_dep1 _ _ _ _ _ _ H) => H0 H1.
+    apply (eq_ind y (fun p0 : P p => x = p0 -> x = y) (fun H0 : x = y => H0)
+                  (eq_rect p P y p H0) (eqType_eq_rect_eq U P p y H0) H1
+          ).
+  Qed.
+  Lemma eq_existT : forall (U : eqType) P (p : U) (x y : P p),
+                      existT P p x = existT P p y -> x = y.
+  Proof.
+    move=> U P p x y H.
+    move: (eq_ind (existT P p y) (fun s : sigT P => EqdepFacts.eq_dep U P (projT1 s) (projT2 s) p y) (EqdepFacts.eq_dep_intro U P p y) (existT P p x) (Logic.eq_sym H)).
+    rewrite /= .
+    move=> H0.
+    apply (eqType_eq_dep_eq _ _ _ _ _ H0).
+  Qed.
+
+
   Notation "'!' a" := (@func 1 e_neg [a]) (at level 35, right associativity).
   Notation "'c' z" := (@func 0 (const z) []) (at level 20).
 
   Inductive program : Set :=
-  | asgn : forall n, V n -> t E n -> E -> program
+  | asgn : forall n, V n -> n.-tuple E -> E -> program
   | skip : program
   | sync : program
   | seq : program -> program -> program
@@ -93,290 +196,193 @@ Section SIMT_Definition.
   Notation "P ;; Q" := (seq P Q) (at level 150).
   Notation "'IFB' e 'THEN' P 'ELSE' Q" := (P_if e P Q) (at level 135).
   Notation "'WHILE' e 'DO' P" := (P_while e P) (at level 140).
-  
-  Definition T := { n : nat & (n < N)%nat}.
 
-  Definition T_S : forall n,
-                   {n0 : nat & (n0 < n)%nat} ->
-                   {n0 : nat & (n0 < S n)%nat}.
-    intros. destruct H. exists x. abstract omega.
-  Defined.
+  Definition T := 'I_N. (* The set of threads *)
+  Definition T_eqType := ordinal_eqType N.
+  Definition T_finType := ordinal_finType N.
 
-  Lemma T_dec : forall (P : T -> Prop),
-                  (forall i, P i \/ ~ P i) ->
-                  (forall i, ~ P i) \/ (exists i, P i).
-    unfold T.
-    induction N; intros.
-    - left. intros. inversion i.
-      induction x; inversion H0.
-    - set (P' (u : {n0 : nat & (n0 < n)%nat}) := P (T_S _ u)).
-      destruct (IHn P').
-      + firstorder.
-      + unfold P' in *.
-        assert ((n < S n)%nat) by omega.
-        destruct (H (exist _ n H1)).
-        * right. eexists. eassumption.
-        * left. intros.
-          destruct i.
-          inversion l; subst.
-          { rewrite <- (proof_irrelevance _ H1 l). assumption. }
-          { apply le_S_gt in H4.
-            assert (exists i : {n0 : nat & (n0 < n)%nat},
-                      T_S _ i = existT (fun n0 : nat => (n0 < S n)%nat) x l).
-            exists (existT _ x H4).
-            simpl.
-            apply f_equal.
-            apply proof_irrelevance.
-            destruct H3.
-            rewrite <- H3.
-            apply H0.
-          }
-      + destruct H0.
-        right. exists (T_S _ x). assumption.
-  Qed.
-
-  Definition L_map n := T -> t Z n -> Z.
-  Definition S_map n := t Z n -> Z.
+  Definition L_map n := T -> n.-tuple int -> int.
+  Definition S_map n := n.-tuple int -> int.
   Definition state := ((forall n, LV n -> L_map n) * (forall n, SV n -> S_map n))%type.
 
   Reserved Notation "s '[[' e ']](' i ')'" (at level 50).
 
-  Fixpoint E_under_state (s:state) e : T -> Z :=
+  Fixpoint E_under_state (s:state) e : T -> int :=
     match e with
-      | tid => fun t => match t with existT i _ => Z.of_nat i end
-      | ntid => fun _ => Z.of_nat N
-      | var n (inl lv) es =>
-        fun i => fst s n lv i (map (fun e => s[[e]](i)) es)
-      | var n (inr sv) es =>
-        fun i => snd s n sv (map (fun e => s[[e]](i)) es)
+      | tid => id
+      | ntid => fun _ => N
+      | var n (local_variable lv) es =>
+        fun i => s.1 n lv i (tuple_of_Vector (Vector.map (fun e => s[[e]](i)) es))
+      | var n (shared_variable sv) es =>
+        fun i => s.2 n sv (tuple_of_Vector (Vector.map (fun e => s[[e]](i)) es))
       | func n f es =>
-        fun i => f (map (fun e => s[[e]](i)) es)
+        fun i => f (tuple_of_Vector (Vector.map (fun e => s[[e]](i)) es))
     end
       where "s '[[' e ']](' i ')'" := (E_under_state s e i).
 
-  Definition Zeq_list_bool n (zs zs' : t Z n) :=
-    fold_left (fun b b' => andb b b') true
-              (map2 (fun z z' => Zeq_bool z z') zs zs').
+  Definition update n (f : n.-tuple int -> int) zs z :=
+    fun zs' => if zs == zs' then z else f zs'.
 
-  Definition update n (f : t Z n -> Z) (zs : t Z n) (z : Z) :=
-    fun zs' : t Z n => if Zeq_list_bool n zs zs' then z else f zs'.
-
-  Definition update_state (s : state) n (x : V n) (x' : (T -> t Z n -> Z) + (t Z n -> Z)) : state.
-    refine (
-        match x, x' with
-          | inl lv, inl lv' =>
-            ((fun n0 (lv0 : LV n0) =>
-                match eq_nat_dec n n0 return L_map n0 with
-                  | left e => _
-                  | right _ => fst s n0 lv0
-                end), snd s)
-          | inr sv, inr sv' =>
-            (fst s,
-             fun n0 (sv0 : SV n0) =>
-               match eq_nat_dec n n0 return S_map n0 with
-                 | left e => _
-                 | right _ => snd s n0 sv0
-               end)
-          | _, _ => s
-        end
-      ).
-    - clear x x'. subst.
-      refine (if eq_lv_dec _ lv lv0 then fun i => fun zs => lv' i zs else fst s _ lv0).
-    - clear x x'. subst.
-      refine (if eq_sv_dec _ sv sv0 then sv' else snd s _ sv0).
+  Definition update_state (s : state) n (x : V n) (x' : (T -> n.-tuple int -> int) + (n.-tuple int -> int)) : state.
+    destruct x; destruct x'; [|exact s|exact s|].
+    {
+      refine ((fun n0 (lv0 : LV n0) => _, s.2)).
+      case: (@eqnP n n0) => H.
+      { subst. exact (if l == lv0 then i else s.1 _ lv0). }
+      { exact (s.1 n0 lv0). }
+    }
+    {
+      refine (s.1, (fun n0 (sv0 : SV n0) => _)).
+      case: (@eqnP n n0) => H.
+      { subst. exact (if s0 == sv0 then i else s.2 _ sv0). }
+      { exact (s.2 n0 sv0). }
+    }
   Defined.
-
   Transparent update_state.
 
-  Definition mask := T -> bool.
-  Definition empty : mask := fun _ => false.
-  Definition T_mask : mask := fun _ => true.
+  Ltac unfold_update_state :=
+    match goal with
+      | [ H : context[update_state]|-_] => rewrite/update_state in H
+      | [ |- context[update_state]] => rewrite/update_state
+      | _ => fail
+    end.
+  Ltac simplify_update_state' :=
+    match goal with
+      | [ H : context[eq_rect_r] |- _] => rewrite/eq_rect_r in H
+      | [ H : context[eq_rec_r] |- _] => rewrite/eq_rec_r in H
+      | [ H : context[eq_rect ?x _ _ _ _ _ _] |- _] =>
+        destruct (@eqnP x x); rewrite // in H;
+        rewrite (eq_irrelevance (Logic.eq_sym _) erefl)
+      | [ H : context[eq_rec ?x _ _ _ _ _ _] |- _] =>
+        destruct (@eqnP x x); rewrite // in H;
+        rewrite (eq_irrelevance (Logic.eq_sym _) erefl)
+      | [ |- context[eq_rect_r]] => rewrite/eq_rect_r
+      | [ |- context[eq_rec_r]] => rewrite/eq_rec_r
+      | [ |-context[eq_rect ?x _ _ _ _ _ _]] =>
+        destruct (@eqnP x x); rewrite //;
+                                      rewrite (eq_irrelevance (Logic.eq_sym _) erefl)
+      | [ |-context[eq_rec ?x _ _ _ _ _ _]] =>
+        destruct (@eqnP x x); rewrite //;
+                                      rewrite (eq_irrelevance (Logic.eq_sym _) erefl)
+      | [ |-context[eqnP]] =>
+        case: eqnP => //=
+      | _ => fail
+    end.
+  Ltac simplify_update_state :=
+    repeat unfold_update_state; simpl; repeat simplify_update_state'; simpl.
 
-  Definition meet (mu mu' : mask) : mask := fun i => andb (mu i) (mu' i).
-  Definition diff (mu mu' : mask) : mask := fun i => andb (mu i) (negb (mu' i)).
+  Definition mask := {set T}.
+  Definition empty : mask := set0.
+  Definition T_mask : mask := [set: T].
+  Definition T_pred := set_predType T_finType.
 
-  Definition sub (mu mu' : mask) : Prop :=
-    forall i : T, mu i = true -> mu' i = true.
-
-  Lemma fold_meet : forall mu mu', (fun i => (mu i && mu' i))%bool = meet mu mu'.
-  Proof.
-    reflexivity.
-  Qed.
-
-  Lemma meet_empty_l : forall m, meet empty m = empty.
-  Proof.
-    intros; unfold meet, empty; apply functional_extensionality;
-    intro;
-    destruct (m x); try reflexivity.
-  Qed.
-
-  Lemma meet_empty_r : forall m, meet m empty = empty.
-  Proof.
-    intros; unfold meet, empty; apply functional_extensionality;
-    intro;
-    destruct (m x); try reflexivity.
-  Qed.
-
-  Lemma meet_comm : forall m m', meet m m' = meet m' m.
-  Proof.
-    intros; unfold meet, empty; apply functional_extensionality;
-    intro;
-    destruct (m x); destruct (m' x); try reflexivity.
-  Qed.
-
-  Lemma meet_assoc : forall m m' m'', meet (meet m m') m'' =
-                                      meet m (meet m' m'').
-  Proof.
-    intros; unfold meet, empty; apply functional_extensionality;
-    intro;
-    destruct (m x); destruct (m' x); destruct (m'' x); try reflexivity.
-  Qed.
-
-  Lemma meet_double : forall m, meet m m = m.
-  Proof.
-    intros; unfold meet, empty; apply functional_extensionality;
-    intro;
-    destruct (m x); try reflexivity.
-  Qed.
-
-  Lemma sub_meet : forall m m', sub m m' -> meet m m' = m.
-  Proof.
-    intros.
-    apply functional_extensionality; intro i.
-    unfold sub in H.
-    generalize (H i); clear H; intro.
-    unfold meet.
-    destruct (m i); destruct (m' i); try reflexivity.
-    generalize (H (refl_equal _)); intro H'; inversion H'.
-  Qed.
-
-  Definition s_es n s := fun (es : t E n) i => map (fun e => s[[e]](i)) es.
+  Definition s_es n s := fun (es : n.-tuple E) i =>
+                           [tuple of [seq s[[e]](i) | e <- es]].
   Notation "s '[[[' es ']]](' i ')'" := (s_es _ s es i) (at level 50).
 
   Inductive eval : program -> mask -> state -> state -> Prop :=
   | E_Inactive : forall P s, eval P empty s s
   | E_Skip : forall mu s, eval skip mu s s
   | E_Sync : forall s, eval sync T_mask s s
-  | E_LAssign : forall n (x : LV n) es e mu (s s' : state),
-                  snd s' = snd s ->
+  | E_LAssign : forall n (x : LV n) es e (mu : mask) (s s' : state),
+                  (forall n, s'.2 n =2 s.2 n) ->
                   (forall n',
-                     if eq_nat_dec n n' then
+                     if n == n' then
                        forall y : LV n,
-                         if eq_lv_dec _ x y then
-                           (forall i, mu i = false -> fst s' n x i = fst s n x i) /\
-                           (forall i, mu i = true ->
-                                      fst s' n x i =
-                                      update n (fst s n x i) (s[[[es]]](i)) (s[[e]](i))
-                           )
-                         else fst s' n y = fst s n y
-                     else (forall y : LV n', fst s' n' y = fst s n' y)) ->
-                  eval (asgn (inl x) es e) mu s s'
-  | E_SAssign : forall n (x : SV n) es e mu (s s' : state),
-                  fst s' = fst s ->
+                         if x == y then
+                           forall i : T,
+                             s'.1 n x i =1
+                             if i \in mu then
+                               update n (s.1 n x i) (s[[[es]]](i)) (s[[e]](i))
+                             else
+                               s.1 n x i
+                         else s'.1 n y =2 s.1 n y
+                     else (forall y : LV n', s'.1 n' y =2 s.1 n' y)) ->
+                  eval (asgn x es e) mu s s'
+  | E_SAssign : forall n (x : SV n) es e (mu : mask) (s s' : state),
+                  (forall n (lv : LV n), s'.1 n lv =2 s.1 n lv) ->
                   (forall n',
-                     if eq_nat_dec n n' then
+                     if n == n' then
                        forall y : SV n,
-                         if eq_sv_dec _ x y then
+                         if x == y then
                            (forall ns,
-                              ((forall i, mu i = true ->
-                                          Zeq_list_bool _ (s[[[es]]](i)) ns = false) ->
-                               snd s' n x ns = snd s n x ns) /\
-                              ((exists i, mu i = true /\
-                                          Zeq_list_bool _ (s[[[es]]](i)) ns = true) ->
-                               (exists j, mu j = true /\
-                                          Zeq_list_bool _ (s[[[es]]](j)) ns = true /\
-                                          snd s' n x ns = (s[[e]](j))))
+                              if [forall (i | i \in mu), s[[[es]]](i) != ns] then
+                                s'.2 n x ns = s.2 n x ns
+                              else
+                                [exists (i | i \in mu),
+                                   (s[[[es]]](i) == ns)
+                                     && (s'.2 n x ns == s[[e]](i))]
                            )
-                         else snd s' n y = snd s n y
-                     else (forall y : SV n', snd s' _ y = snd s _ y)) ->
-                  eval (asgn (inr x) es e) mu s s'
+                         else s'.2 n y =1 s.2 n y
+                     else (forall y : SV n', s'.2 _ y =1 s.2 _ y)) ->
+                  eval (asgn x es e) mu s s'
   | E_Seq : forall P Q mu s s' s'', eval P mu s s' ->
                                     eval Q mu s' s'' ->
                                     eval (seq P Q) mu s s''
-  | E_If : forall P Q mu s e s_e s' s'',
-             s_e = (fun i => negb (Zeq_bool (s[[e]](i)) 0)) ->
-             eval P (meet mu s_e) s s' ->
-             eval Q (diff mu s_e) s' s'' ->
+  | E_If : forall P Q (mu : mask) s e (s_e : mask) s' s'',
+             s_e = [set i | bool_of_int (s[[e]](i))] ->
+             eval P (mu :&: s_e) s s' ->
+             eval Q (mu :\: s_e) s' s'' ->
              eval (IFB e THEN P ELSE Q) mu s s''
-  | E_While : forall P mu s e mu' s' s'',
-                mu' = meet mu (fun i => negb (Zeq_bool (s[[e]](i)) 0)) ->
+  | E_While : forall P (mu : mask) s e mu' s' s'',
+                mu' = mu :&: [set i | bool_of_int (s[[e]](i))] ->
                 eval P mu' s s' ->
                 eval (WHILE e DO P) mu' s' s'' ->
                 eval (WHILE e DO P) mu s s''.
 
   Definition assertion := state -> Prop.
 
-  Definition mask_of (m : T -> Z) i : bool := negb (Zeq_bool (m i) 0%Z).
+  Definition mask_of (m : T -> int) : mask := [set i | bool_of_int (m i)].
 
-  Lemma fold_mask_of : forall m, (fun i => negb (Zeq_bool (m i) 0%Z)) = mask_of m.
-    reflexivity.
-  Qed.
-
-  Lemma meet_equiv :
+  Lemma setI_e_and :
     forall m z,
-      meet (mask_of m) (mask_of z) = mask_of (fun i => e_and [m i; z i]).
+       (mask_of m) :&: (mask_of z) = mask_of (fun i => e_and [tuple m i; z i]).
   Proof.
-    intros m z; apply functional_extensionality; intro i;
-    unfold meet, mask_of; unfold negb;
-    destruct (m i); simpl; destruct (z i); try reflexivity.
+    move => m z.
+    apply setP => i.
+    rewrite /mask_of/e_and -setIdE 3!in_set int_of_boolK // .
   Qed.
 
-  Lemma diff_equiv :
+  Lemma setD_e_and_neg :
     forall m z,
-      diff (mask_of m) (mask_of z) = mask_of (fun i => e_and [m i; e_neg [z i]]).
+      (mask_of m) :\: (mask_of z) = mask_of (fun i => e_and [tuple m i; e_neg [tuple z i]]).
   Proof.
-    intros m z; apply functional_extensionality; intro i;
-    unfold diff, mask_of; unfold negb.
-    destruct (m i); simpl; destruct (z i); try reflexivity.
+    move => m z.
+    apply setP => i.
+    rewrite /mask_of/e_and/e_neg/= setDE -setIdE 4!in_set 2!int_of_boolK // .
   Qed.
-
-  Ltac simplify_mask' :=
-    match goal with
-      | [ H : context[mask_of] |- _] => unfold mask_of in H
-      | [ H : context[meet] |- _] => unfold meet in H
-      | [ H : context[diff] |- _] => unfold diff in H
-      | [ H : context[negb] |- _] => unfold negb in H
-      | _ => fail
-    end.
-
-  Ltac simplify_mask := repeat simplify_mask'; simpl in *|-*.
-
   Definition hoare_quadruple (phi : assertion) m (P : program) (psi : assertion) : Prop :=
     forall s s' : state,
       phi s ->
       eval P (mask_of m) s s' ->
       psi s'.
 
-  Definition all e := forall i : T, e i <> 0%Z.
-  Definition none e := forall i : T, e i = 0%Z.
-  Definition forall_in_mask (s : state) m (P : T -> Prop) :=
-    forall i : T, m i <> 0%Z -> P i.
-  Definition exists_in_mask (s : state) m (P : T -> Prop) :=
-    exists i : T, m i <> 0%Z /\ P i.
+  Definition all (e : T -> int) := forall i : T, e i != 0.
+  Definition none (e : T -> int) := forall i : T, e i == 0.
 
-  Definition lassign (s : state) n (x' : T -> t Z n -> Z) m (x : LV n) (es : t E n) (e : E) : Prop :=
-    forall (ns : t Z n) (i : T),
-      (m i = 0%Z \/ Zeq_list_bool _ (s[[[es]]](i)) ns = false ->
+  Definition lassign (s : state) n (x' : T -> n.-tuple int -> int) (m : T -> int) (x : LV n) (es : n.-tuple E) (e : E) : Prop :=
+    forall (ns : n.-tuple int) (i : T),
+      (m i == 0 \/ s[[[es]]](i) != ns ->
        (x' i ns = fst s n x i ns)) /\
-      (m i <> 0%Z /\ Zeq_list_bool _ (s[[[es]]](i)) ns = true ->
+      (m i != 0 /\ s[[[es]]](i) == ns ->
        (x' i ns = s[[e]](i))).
 
-  Definition sassign s n (x' : t Z n -> Z) m (x : SV n) (es : t E n) (e : E) : Prop :=
-    (forall ns : t Z n,
-       (forall_in_mask s m (fun i => Zeq_list_bool _ (s[[[es]]](i)) ns = false) /\
-       x' ns = snd s n x ns) \/
-       (exists_in_mask s m (fun i => Zeq_list_bool _ (s[[[es]]](i)) ns = true /\
-                                    x' ns = s[[e]](i)))).
+  Definition sassign s n (x' : n.-tuple int -> int) (m : T -> int) (x : SV n) (es : n.-tuple E) (e : E) : Prop :=
+    (forall ns : n.-tuple int,
+       ([forall (i | i \in mask_of m), s[[[es]]](i) != ns] /\
+        x' ns = snd s n x ns) \/
+       ([exists (i | i \in mask_of m),
+           (s[[[es]]](i) == ns) && (x' ns == s[[e]](i))])).
 
-  Definition assign rho n x' m (x : V n) (es : t _ n) (e : _) :=
+  Definition assign rho n x' (m : T -> int) (x : V n) (es : n.-tuple _) (e : _) :=
     match x, x' return Prop with
-      | inl lv, inl lv' => lassign rho n lv' m lv es e
-      | inr sv, inr sv' => sassign rho n sv' m sv es e
+      | local_variable lv, inl lv' => lassign rho n lv' m lv es e
+      | shared_variable sv, inr sv' => sassign rho n sv' m sv es e
       | _, _ => False
     end.
   Implicit Arguments assign [n].
 
-  Inductive Hoare_proof : assertion -> (T -> Z) -> program -> assertion -> Prop :=
+  Inductive Hoare_proof : assertion -> (T -> int) -> program -> assertion -> Prop :=
   | H_Skip : forall phi m, Hoare_proof phi m skip phi
   | H_Sync : forall (phi : assertion) m,
                Hoare_proof (fun s => (all m \/ none m) -> phi s)
@@ -390,334 +396,302 @@ Section SIMT_Definition.
               Hoare_proof phi m P psi ->
               Hoare_proof psi m Q chi ->
               Hoare_proof phi m (P ;; Q) chi
-  | H_Assign : forall n (x : V n) (es : t E n) e m (phi : assertion),
+  | H_Assign : forall n (x : V n) (es : n.-tuple E) e m (phi : assertion),
                  Hoare_proof (fun s =>
                                 forall x', assign s x' m x es e ->
                                            phi (update_state s n x x'))
                              m (asgn x es e) (fun s => phi s)
-  | H_If : forall (phi : assertion) psi chi e (m : T -> Z) P Q,
-             (forall z : T -> Z,
+  | H_If : forall (phi : assertion) psi chi e (m : T -> int) P Q,
+             (forall z : T -> int,
                 Hoare_proof
                   (fun s =>
                      phi s /\
                      (forall i, s[[e]](i) = z i))
-                  (fun i => e_and [m i; z i]) P (psi z)) ->
-             (forall z, Hoare_proof (psi z) (fun i => e_and [m i; e_neg [z i]]) Q chi) ->
+                  (fun i => e_and [tuple m i; z i]) P (psi z)) ->
+             (forall z, Hoare_proof (psi z) (fun i => e_and [tuple m i; e_neg [tuple z i]]) Q chi) ->
              Hoare_proof phi m (IFB e THEN P ELSE Q) chi
   | H_While : forall (phi : assertion) m e P,
-                (forall z : T -> Z,
-                   Hoare_proof (fun s => phi s /\ (forall i, s[[e]](i) = z i)) (fun i => e_and [m i; z i]) P phi) ->
-                Hoare_proof phi m (WHILE e DO P) (fun s => phi s /\ none (fun i : T => e_and [m i; s[[e]](i)])).
+                (forall z : T -> int,
+                   Hoare_proof (fun s => phi s /\ (forall i, s[[e]](i) = z i)) (fun i => e_and [tuple m i; z i]) P phi) ->
+                Hoare_proof phi m (WHILE e DO P) (fun s => phi s /\ none (fun i : T => e_and [tuple m i; s[[e]](i)])).
 
-  Lemma lem_1 : forall s s' n (x : V n) es e (m : T -> Z),
+  Lemma lem_1 : forall s s' n (x : V n) es e (m : T -> int),
                    eval (asgn x es e) (mask_of m) s s' <->
                    exists a,
                        s' = update_state s _ x a /\
                        assign s a m x es e.
   Proof.
     split; intros.
-    - (* => *)
-      inversion H; subst; clear H.
-      + destruct x as [lv | sv].
-        * destruct s'.
-          exists (inl (fun i => fun zs => l n lv i zs)).
-          simpl.
+    { inversion H; subst; clear H.
+      {
+        destruct x as [lv | sv].
+        {
+          destruct s'.
+          exists (inl (l n lv)).
+          simplify_update_state.
           split.
-          { functional_extensionality_dep_pair_r; intro n'.
-            destruct (eq_nat_dec n n'); try reflexivity; subst.
-            unfold eq_rec_r. unfold eq_rec. unfold eq_rect.
+          { functional_extensionality_dep_pair_r => n'.
+            simplify_update_state => p.
             subst.
-            simpl.
-            rewrite <- functional_extensionality with (f:=l n');
-              try reflexivity; intro lv'.
-            destruct (eq_lv_dec _ lv lv'); try reflexivity.
-            subst.
-            reflexivity. }
-          { unfold lassign. intros. split.
-            - apply equal_f with (x:=i) in H2.
-              destruct (m i); reflexivity.
-            - intros. destruct H.
-              apply equal_f with (x:=i) in H2.
-              unfold mask_of in *.
-              destruct (m i); try (unfold mask_of in *; contradict H2;
-                                  discriminate);
-              contradict H; reflexivity. }
-        * destruct s'.
+            simplify_update_state.
+            apply functional_extensionality => lv'.
+            case:ifP => H // .
+            rewrite (elimT eqP H) //= . }
+          { rewrite/lassign => ns i.
+            split => //= .
+            (do 2!case/andP) => H _.
+            apply setP in H2.
+            rewrite /empty/mask_of/bool_of_int in H2.
+            move: (H2 i).
+            rewrite in_set0 in_set H// . }}
+        { destruct s'.
           exists (inr (fun zs => s n sv zs)).
-          simpl.
           split.
-          { functional_extensionality_dep_pair_r; intro n'.
-            destruct (eq_nat_dec n n'); try reflexivity; subst.
-            unfold eq_rec_r. unfold eq_rec. unfold eq_rect.
+          { simplify_update_state.
+            functional_extensionality_dep_pair_r => n'.
+            simplify_update_state => p.
             subst.
-            simpl.
-            rewrite <- functional_extensionality with (f:=s n');
-              try reflexivity; intro sv'.
-            destruct (eq_sv_dec _ sv sv'); try reflexivity.
-            subst.
-            reflexivity. }
-          { unfold sassign. intros.
-            unfold mask_of in *.
-            unfold forall_in_mask. unfold exists_in_mask.
+            apply functional_extensionality => sv'.
+            simplify_update_state.
+            case:ifP => H // .
+            rewrite (elimT eqP H) //= . }
+          { rewrite/sassign => ns.
             left.
-            split; intros.
-            apply equal_f with (x:=i) in H2;
-            destruct (m i); try (contradict H; reflexivity);
-            try (contradict H2; discriminate). reflexivity. }
-      + existT_eq.
+            split => //= .
+            apply setP in H2.
+            rewrite /empty/mask_of/bool_of_int in H2.
+            apply (introT forall_inP) => i.
+            move: (H2 i).
+            rewrite in_set0 in_set.
+            move => H.
+              by rewrite -H. }
+        }
+      }
+      { move: (eq_existT _ _ _ _ _ H1) => {H1} H1.
+        move: (eq_existT _ _ _ _ _ H3) => {H3} H3.
         destruct s. destruct s' as [l' s'].
-        simpl in H8.
-        unfold update_state.
-        unfold eq_rec_r. unfold eq_rec. unfold eq_rect.
-        simpl in H7. subst.
-        simpl.
-        eexists (inl _).
+        rewrite /= in H7,H8|-*.
+        subst.
+        eexists (inl (l' n _)).
         split.
-        * functional_extensionality_dep_pair_r; try reflexivity.
-          intro n'.
-          generalize (H8 n'); intro H8'; clear H8.
-          destruct (eq_nat_dec n n'); subst; try reflexivity.
-          rewrite <- functional_extensionality with (f:=l' n');
-            try reflexivity.
-          subst. intro lv'.
-          simpl.
-          generalize (H8' lv'); intro H8; clear H8'.
-          destruct (eq_lv_dec _ x1 lv'); subst; try reflexivity; assumption.
-          apply functional_extensionality. intros. apply H8'.
-        * unfold lassign.
+        { simplify_update_state.
+          rewrite /eqrel in H7.
+          assert ((l', s') = (l', s)).
+          { functional_extensionality_dep_pair_r => n'.
+            apply functional_extensionality => sv.
+            apply functional_extensionality => y.
+            rewrite (H7 _ sv y) => // . }
+          rewrite H.
+          functional_extensionality_dep_pair_r => n'.
+          simplify_update_state => p.
+          { subst.
+            move: (H8 n') => {H8}.
+            case: (@eqnP n' n') => p.
+            { rewrite (introT eqP p).
+              move => H8.
+              apply functional_extensionality => lv.
+              move: (H8 lv) => {H8}.
+              case: (lv_eqP _ x1 lv) => H0.
+              { rewrite (introT eqP H0) /= .
+                subst.
+                case: ifP => // H1.
+                  by apply (elimF eqP) in H1. }
+              { apply (introF eqP) in H0.
+                simplify_update_state.
+                rewrite H0 => H1.
+                apply functional_extensionality => i.
+                apply functional_extensionality => // . }}
+            { rewrite (introF eqP p).
+              simplify_update_state => // . }}
+          { move: (H8 n').
+            rewrite (introF eqP p) => H0.
+            apply functional_extensionality => lv // .
+            apply functional_extensionality => i.
+            apply functional_extensionality => x.
+            rewrite (H0 lv i x) => // . }}
+        { rewrite /=/lassign.
           intros.
-          generalize (H8 n); intro H8'; clear H8.
-          destruct (eq_nat_dec n n) as [H|H]; [|contradict H; reflexivity].
-          generalize (H8' x1); intro H8; clear H8'.
-          destruct (eq_lv_dec _ x1 x1); [|contradict n0; reflexivity].
-          simplify_mask.
-          destruct H8 as [H0 H1].
-          generalize (H0 i); intro H0'; clear H0.
-          generalize (H1 i); intro H1'; clear H1.
-          simpl. split.
-          { intros.
-            destruct (m i); try (simpl in H0'; rewrite H0'; reflexivity);
-            simpl in H1';
-            destruct H0; try discriminate;
-            rewrite H1'; try reflexivity;
-            unfold update; rewrite H0; reflexivity. }
-          { intros. destruct H0.
-            destruct (m i);
-              try (rewrite H1'; try reflexivity;
-                   unfold update; rewrite H1; reflexivity);
-              contradict H0; reflexivity. }
-      + existT_eq.
+          move: (H8 n) => {H8} H8.
+          rewrite (introT eqP erefl) in H8.
+          move: (H8 x1) => {H8} H8.
+          rewrite (introT eqP erefl) in H8.
+          rewrite /= .
+          rewrite (H8 i) => {H8}.
+          rewrite /mask_of/bool_of_int in_set.
+          case:ifP => /= H; split => // => H0.
+          { rewrite (negbTE H) in H0.
+            case: H0 => // H0.
+            rewrite /update.
+            case:ifP => // .
+            rewrite (negbTE H0) // . }
+          { case: H0 => H0 H1.
+            rewrite /update.
+            case:ifP => // .
+            rewrite H1 // . }
+          { case H0 => // . }
+        }
+      }
+      { move: (eq_existT _ _ _ _ _ H1).
+        move: (eq_existT _ _ _ _ _ H3).
+        move => {H1} {H3} H1 H3.
         destruct s. destruct s' as [l' s'].
-        simpl in H8.
-        unfold update_state.
-        unfold eq_rec_r. unfold eq_rec. unfold eq_rect.
-        simpl in H7. subst.
-        simpl.
+        rewrite /= in H7,H8|-*.
+        simplify_update_state.
+        rewrite /= .
+        subst.
         eexists (inr _).
         split.
-        functional_extensionality_dep_pair_r; try reflexivity.
-          intro n'.
-          generalize (H8 n'); intro H8'; clear H8.
-          destruct (eq_nat_dec n n'); subst; try reflexivity.
-          rewrite <- functional_extensionality with (f:=s' n'); try reflexivity.
-          subst. intro sv'.
-          simpl.
-          generalize (H8' sv'); intro H8; clear H8'.
-          destruct (eq_sv_dec _ x1 sv'); subst; try reflexivity; assumption.
-          apply functional_extensionality. intro. apply H8'.
-        * unfold sassign.
-          intros.
-          generalize (H8 n); intro H8'; clear H8.
-          destruct (eq_nat_dec n n) as [H|H]; [|contradict H; reflexivity].
-          generalize (H8' x1); intro H8; clear H8'.
-          destruct (eq_sv_dec _ x1 x1); [|contradict n0; reflexivity].
-          simplify_mask.
-          unfold forall_in_mask.
-          unfold exists_in_mask.
-          destruct (H8 ns) as [H0 H1]; clear H8.
-          destruct T_dec
-          with (P:=(fun i =>
-                      negb (Zeq_bool (m i) 0) = true /\
-                      Zeq_list_bool _ ((l,s)[[[es]]](i)) ns = true)).
-          { unfold not. intros.
-            destruct (m i); simpl;
-            try (right; intros; destruct H2; inversion H2; fail);
-            destruct (Zeq_list_bool n ((l,s)[[[es]]](i)));
-            try (left; split; reflexivity);
-            right; intros; destruct H2; discriminate.
+        { rewrite /eqrel in H7.
+          assert ((l', s') = (l, s')).
+          { functional_extensionality_dep_pair_r => n'.
+            apply functional_extensionality => lv'.
+            apply functional_extensionality => i.
+            apply functional_extensionality => ns.
+            rewrite (H7 _ _ _ _) // . }
+          rewrite H.
+          functional_extensionality_dep_pair_r => n'.
+          rewrite /eqfun in H8.
+          simplify_update_state => p.
+          { subst.
+            move: (H8 n') => {H8}.
+            case: (@eqnP n' n') => p.
+            { rewrite (introT eqP p).
+              subst.
+              move => H8.
+              apply functional_extensionality => sv.
+              move: (H8 sv) => {H8}.
+              case: (sv_eqP _ x1 sv) => H0.
+              { rewrite (introT eqP H0) /= .
+                subst.
+                move=> H0.
+                rewrite (introT eqP erefl) => // . }
+              { apply (introF eqP) in H0.
+                simplify_update_state.
+                rewrite H0 => H1.
+                apply functional_extensionality => // . }}
+            { rewrite (introF eqP p).
+              simplify_update_state => // . }}
+          { move: (H8 n').
+            rewrite (introF eqP p) => H0.
+            apply functional_extensionality => sv // .
+            apply functional_extensionality => i.
+            rewrite (H0 sv i) => // . }}
+        { rewrite/=/sassign => ns.
+          move: (H8 n) => {H8} H8.
+          rewrite (introT eqP erefl) in H8.
+          move: (H8 x1) => {H8} H8.
+          rewrite (introT eqP erefl) in H8.
+          move: (H8 ns).
+          rewrite /mask_of/bool_of_int/= => {H8}.
+          case:ifP => H H0; try by right.
+          left.
+          split => // .
+        }
+      }
+    }
+    { (* <= *)
+      destruct x as [lv | sv]; constructor;
+      case: H;
+      case => [la | sa]; case; case s; case s' => {s} {s'} l s l' s';
+        case => H H0 H1; subst => //= n'.
+      { case: ifP => H0 y.
+        {
+          apply (elimT eqP) in H0.
+          subst.
+          simplify_update_state.
+          case: ifP => H2 i.
+          { apply (elimT eqP) in H2.
+            subst.
+            rewrite /=/lassign in H1.
+            rewrite /mask_of/update/bool_of_int/eqfun/= => ns.
+            rewrite (introT eqP erefl).
+            move: (H1 ns i) => {H1}.
+            rewrite /= .
+            case => H H0.
+            rewrite in_set.
+            case:ifP => // => H2.
+            { case:ifP => H3.
+              { rewrite H0 => //= . }
+              { rewrite H3/negb in H0.
+                rewrite H => // .
+                rewrite H3/negb.
+                  by right. }
+            }
+            { apply negbT in H2.
+              rewrite negbK in H2.
+              rewrite H2 in H0.
+              rewrite H => // .
+                by left. }
           }
-          { left.
-            split.
-            - intros. generalize (H2 i); intro H2'.
-              destruct (m i); try (contradict H3; reflexivity);
-              destruct (Zeq_list_bool n ((l,s)[[[es]]](i)));
-                try (destruct H2'; split; reflexivity); reflexivity.
-            - apply H0. intros.
-              generalize (H2 i); intro H2'.
-              destruct (m i); try discriminate;
-              destruct (Zeq_list_bool n ((l,s)[[[es]]](i)));
-                try (simpl in H2'; destruct H2'; split; reflexivity);
-                reflexivity.
+          { move=> ns.
+              by rewrite H2. }}
+        { simplify_update_state => p.
+            by rewrite (introT eqP p) in H0. }}
+      { case: ifP => H0 y.
+        { apply (elimT eqP) in H0.
+          subst.
+          case:ifP => // H2 ns.
+          { apply (elimT eqP) in H2.
+            subst.
+            simplify_update_state.
+            move: (H1 ns) => {H1}.
+            case => H0.
+            { case: H0 => H0 H1.
+              rewrite H0.
+              case:ifP => // . }
+            { assert [exists i in mask_of m, ~~((l',s')[[[es]]](i) != ns)].
+              { move: H0; clear => H0.
+                apply (introT existsP).
+                apply (elimT existsP) in H0.
+                case: H0 => i H0.
+                exists i.
+                apply/andP.
+                move/andP in H0.
+                case: H0 => H0.
+                move/andP.
+                case => H1 H2.
+                split => // .
+                apply negbT.
+                  by rewrite H1. }
+              rewrite -negb_forall_in in H.
+              rewrite (negbTE H).
+              rewrite (introT eqP erefl) // . }
           }
-          {
-            right.
-            destruct (H1 H2).
-            exists x.
-            destruct H3 as [H3 [H3' H3'']].
-            repeat split; try assumption.
-            destruct (m x); try (contradict H3; discriminate); try reflexivity.
-          }
-    - (* <= *)
-      destruct x as [lv | sv]; constructor.
-      + destruct H. destruct x as [la | sa].
-        * destruct H. simpl in H0. subst. reflexivity.
-        * destruct H. inversion H0.
-      + destruct H. destruct x as [la | sa].
-        * intros.
-          destruct (eq_nat_dec n n'); subst; try intros y.
-          { destruct (eq_lv_dec _ lv y).
-            - split; intros.
-              + destruct H. subst. simpl.
-                simpl in H1.
-                unfold lassign in H1.
-                simplify_mask.
-                destruct (eq_nat_dec n' n'); try (contradict n; reflexivity).
-                unfold eq_rec_r; unfold eq_rec.
-                rewrite <- (eq_rect_eq_dec eq_nat_dec).
-                destruct (eq_lv_dec _ y y); try (contradict n; reflexivity).
-                destruct s. simpl.
-                apply functional_extensionality. intro zs.
-                destruct (H1 zs i); clear H1. simpl in *.
-                destruct (m i); try inversion H0.
-                apply H. left. reflexivity.
-              + destruct H. subst. simpl.
-                simpl in H1.
-                unfold lassign in H1.
-                simplify_mask.
-                destruct (eq_nat_dec n' n'); try (contradict n; reflexivity).
-                unfold eq_rec_r; unfold eq_rec.
-                rewrite <- (eq_rect_eq_dec eq_nat_dec).
-                destruct (eq_lv_dec _ y y); try (contradict n; reflexivity).
-                destruct s. simpl.
-                apply functional_extensionality. intro zs.
-                destruct (H1 zs i); clear H1. simpl in *.
-                unfold update.
-                destruct (m i); try inversion H0;
-                destruct (Zeq_list_bool _ ((l, s)[[[es]]](i)) zs);
-                  try (apply H2; split; try discriminate; reflexivity);
-                  apply H; right; reflexivity.
-            - destruct H. subst.
-              simpl in H0.
-              destruct s.
-              simpl.
-              unfold eq_rec_r; unfold eq_rec.
-              apply functional_extensionality_dep. intro n''.
-              apply functional_extensionality. intro lv''.
-              destruct (eq_nat_dec n' n'); try reflexivity.
-              rewrite <- eq_rect_eq.
-              destruct (eq_lv_dec _ lv y); try reflexivity. subst.
-              contradict n. reflexivity.
-          }
-          { destruct H. subst. destruct s.
-            simpl.
-            destruct (eq_nat_dec n n'); subst;
-            try (contradict n0; reflexivity).
-            reflexivity.
-          }
-        * intros. simpl in H. destruct H. inversion H0.
-      + destruct H. destruct x as [la | sa].
-        * destruct H. inversion H0.
-        * destruct H. simpl in H0. subst. reflexivity.
-      + destruct H. destruct x as [la | sa].
-        * intros. simpl in H. destruct H. inversion H0.
-        * intros.
-          destruct (eq_nat_dec n n'); subst; try intros y.
-          { destruct (eq_sv_dec _ sv y).
-            - intros.
-              destruct H. subst.
-              simpl in H0. unfold sassign in H0.
-              destruct (H0 ns); clear H0.
-              + destruct H. split.
-                * simpl. intros.
-                  destruct (eq_nat_dec n' n'); try (contradict n; reflexivity).
-                  unfold eq_rec_r; unfold eq_rec.
-                  rewrite <- eq_rect_eq.
-                  destruct (eq_sv_dec _ y y); try (contradict n; reflexivity).
-                  assumption.
-                * intros.
-                  destruct H1.
-                  simplify_mask.
-                  exists x.
-                  destruct H1.
-                  repeat split; try assumption.
-                  unfold forall_in_mask in H.
-                  generalize (H x); intros. clear H.
-                  destruct (m x); try (contradict H1; discriminate; fail);
-                  destruct (Zeq_list_bool _ (s[[[es]]](x)) ns);
-                  try (assert (H' : true = false) by (apply H3; discriminate));
-                  try (assert (H' : false = true) by (apply H2; reflexivity));
-                  try inversion H'.
-              + split.
-                * intros.
-                  destruct H as [i [H [H' H'']]].
-                  generalize (H0 i); clear H0; intro H0.
-                  simplify_mask.
-                  destruct (m i); try (contradict H; reflexivity);
-                  simpl in H0;
-                  generalize (H0 (refl_equal _)); intro;
-                  rewrite H' in H1; discriminate.
-                * intros.
-                  simpl.
-                  destruct (eq_nat_dec n' n'); subst;
-                  try (contradict n; reflexivity);
-                  try (unfold eq_rec_r; unfold eq_rec; rewrite <- eq_rect_eq);
-                  destruct (eq_sv_dec _ y y); try (apply H; discriminate);
-                  try contradict n; try reflexivity.
-                  destruct H.
-                  exists x.
-                  destruct H as [H [H' H'']].
-                  unfold mask_of in *.
-                  repeat split; try assumption.
-                  destruct (m x); try (contradict H; reflexivity); reflexivity.
-            - destruct H. subst.
-              simpl in H0.
-              destruct s.
-              simpl.
-              unfold eq_rec_r; unfold eq_rec.
-              apply functional_extensionality_dep. intro n''.
-              destruct (eq_nat_dec n' n'); try reflexivity.
-              rewrite <- eq_rect_eq.
-              destruct (eq_sv_dec _ sv y); try reflexivity. subst.
-              contradict n. reflexivity.
-          }
-          { destruct H. subst. destruct s.
-            simpl.
-            destruct (eq_nat_dec n n'); subst;
-            try (contradict n0; reflexivity).
-            reflexivity.
-          }
+          { simplify_update_state.
+              by rewrite H2. }
+        }
+        { simplify_update_state => H2.
+            by apply (elimF eqP) in H0. }
+      }
+    }
   Qed.
 
   Definition stable :=
     fun e P =>
       forall (mu : mask) (s s' : state),
         eval P mu s s' ->
-        forall i : T, mu i = false -> s[[e]](i) = s'[[e]](i).
+        forall i : T, i \notin mu -> s[[e]](i) = s'[[e]](i).
 
   Lemma lem_2 : forall e P,
                   stable e P ->
                   forall mu s s',
-                    eval P (meet mu (mask_of (E_under_state s e))) s s' ->
-                    sub (meet mu (mask_of (E_under_state s' e)))
-                        (meet mu (mask_of (E_under_state s e))).
+                    eval P (mu :&: (mask_of (E_under_state s e))) s s' ->
+                    (mu :&: (mask_of (E_under_state s' e)))
+                      \subset (mu :&: (mask_of (E_under_state s e))).
   Proof.
-    unfold sub, stable, meet, negb, mask_of.
-    intros.
-    generalize (H _ _ _ H0 i); intros.
-    destruct (mu i); destruct (s[[e]](i)); simpl in *;
-    try reflexivity;
-    try inversion H1.
-    rewrite <- H2 in H1; inversion H1; reflexivity.
+    move=> e P H mu s s' H0.
+    apply (introT subsetP).
+    move=> i.
+    move: (H _ _ _ H0 i) => {H}.
+    rewrite 4!in_set/bool_of_int.
+    case: (i \in mu) => // .
+    case: (s[[e]](i)) => // .
+    case => // .
+    rewrite eq_refl/negb andbF.
+    case:ifP => // H.
+    move=> H1.
+    move: (introT eqP (H1 erefl)).
+    rewrite eq_sym H // .
   Qed.
 
   Inductive regular : program -> Prop :=
@@ -733,22 +707,24 @@ Section SIMT_Definition.
 
   Lemma lem_5_1 : forall e, all e <-> mask_of e = T_mask.
   Proof.
-    split; intros; unfold all in *; unfold mask_of in *; unfold T_mask in *.
-    - apply functional_extensionality; intro i.
-      generalize (H i); intro H'.
-      destruct (e i); try (contradict H'; reflexivity); reflexivity.
-    - intro. apply equal_f with (x:=i) in H.
-      destruct (e i); discriminate.
+    split; rewrite /all/T_mask/mask_of/bool_of_int => H.
+    { apply setP => i.
+      rewrite in_set in_setT (H i) // . }
+    { apply setP in H => i.
+      move: (H i).
+      rewrite in_set in_setT // . }
   Qed.
 
   Lemma lem_5_2 : forall e, none e <-> mask_of e = empty.
   Proof.
-    split; intros; unfold none in *; unfold mask_of in *; unfold empty in *.
-    - apply functional_extensionality; intro i.
-      generalize (H i); intro H'.
-      destruct (e i); try discriminate; try reflexivity.
-    - intro. apply equal_f with (x:=i) in H.
-      destruct (e i); try discriminate; try reflexivity.
+    split; rewrite /none/empty/mask_of/bool_of_int => H.
+    { apply setP => i.
+      rewrite in_set in_set0 (H i) // . }
+    { apply setP in H => i.
+      move: (H i).
+      rewrite in_set in_set0 => H0.
+      apply negbT in H0.
+      rewrite negbK // in H0. }
   Qed.
 
   Lemma while_stable :
@@ -756,19 +732,14 @@ Section SIMT_Definition.
       stable e P ->
       stable e (WHILE e DO P).
   Proof.
-    intros. unfold stable; intros.
+    rewrite /stable => e P H mu s s' H0 i H1.
     remember (WHILE e DO P) as W.
-    induction H0; inversion HeqW; subst.
-    - reflexivity.
-    - unfold stable in H.
-      assert (forall mu', meet mu mu' i = false) by
-          (intros; unfold meet; rewrite H1; reflexivity).
-      generalize (H _ _ _ H0_ i (H0 (mask_of (E_under_state s e)))).
-      intros.
-      generalize (IHeval2 (refl_equal _) (H0 (mask_of (E_under_state s e)))).
-      intros.
-      rewrite H2, H3.
-      reflexivity.
+    induction H0; inversion HeqW; subst => // .
+    assert (i \in (mu :&:[set i | bool_of_int (s[[e]](i))]) ->
+                  i \in mu).
+    { rewrite in_setI.
+      case/andP => //. }
+    rewrite (H _ _ _ H0_ i (contra H0 H1)) (IHeval2 erefl (contra H0 H1)) // .
   Qed.
 
   Lemma lem_2_while :
@@ -776,152 +747,155 @@ Section SIMT_Definition.
       stable e P ->
       forall mu s s',
         eval (WHILE e DO P) mu s s' ->
-        sub (mask_of (E_under_state s' e)) (mask_of (E_under_state s e)).
+        (mask_of (E_under_state s' e)) \subset (mask_of (E_under_state s e)).
   Proof.
-    unfold sub.
-    intros.
+    rewrite /stable/mask_of/bool_of_int => e P H mu s s' H0.
+    apply (introT subsetP) => i.
     remember (WHILE e DO P) as W.
-    induction H0; inversion HeqW; subst; try assumption.
-    clear IHeval1.
-    generalize (H _ _ _ H0_); intro.
-    rewrite fold_mask_of in *.
-    generalize (while_stable _ _ H _ _ _ H0_0 i); intro.
-    generalize (H0 i); intro.
-    generalize H1 H2 H3; clear; intros.
-    unfold meet in *.
-    remember (mask_of (E_under_state s e) i) as b.
-    destruct b; try reflexivity.
-    unfold mask_of in H1, Heqb.
-    rewrite <- H2, <- H3, <- Heqb in H1;
-      try assumption; try (destruct (mu i); reflexivity).
+    induction H0; inversion HeqW; subst => // {IHeval1} {HeqW}.
+    move: (H _ _ _ H0_ i).
+    move: (while_stable _ _ H _ _ _ H0_0 i).
+    rewrite in_setI 2!in_set/bool_of_int.
+    clear.
+    remember (s[[e]](i) != 0) as b.
+    move: Heqb.
+    case: b => // .
+    rewrite andbF /negb.
+    move=> H H0 H1.
+    case:ifP => // .
+    rewrite -(H0 erefl) -(H1 erefl) => H2.
+    rewrite H2 // in H.
   Qed.
 
   Lemma Soundness_while :
     forall phi e p m,
-      (forall z : T -> Z,
+      (forall z : T -> int,
          regular p ->
          forall s s' : state,
            phi s /\ (forall i : T, s [[e ]]( i) = z i) ->
-           eval p (mask_of (fun i0 : T => e_and [m i0; z i0])) s
+           eval p (mask_of (fun i0 : T => e_and [tuple m i0; z i0])) s
                   s' -> phi s') ->
       regular (WHILE e DO p) ->
       forall s s' m',
-        meet (mask_of m') (mask_of (E_under_state s e)) =
-        meet (mask_of m) (mask_of (E_under_state s e)) ->
+        (mask_of m') :&: (mask_of (E_under_state s e)) =
+        (mask_of m) :&: (mask_of (E_under_state s e)) ->
         eval (WHILE e DO p) (mask_of m') s s' ->
         phi s ->
-        phi s' /\ none (fun i : T => e_and [m' i; s' [[e ]]( i)]).
+        phi s' /\ none (fun i : T => e_and [tuple m' i; s' [[e ]]( i)]).
   Proof.
-    intros phi e p m ? ? s s' m' H2 H1 H3.
-    generalize dependent H2.
-    generalize dependent H3.
+    move=> phi e p m H H0 s s' m' H2 H1 H3.
+    move: H2 H3.
     remember (WHILE e DO p) as W.
     remember (mask_of m') as Mu.
-    generalize dependent m'.
+    move: m' HeqMu.
     induction H1; inversion HeqW; subst; unfold none in *; intros.
-    - symmetry in HeqMu. apply lem_5_2 in HeqMu.
+    { symmetry in HeqMu. apply lem_5_2 in HeqMu.
       split; try assumption; intros.
-      rewrite (HeqMu i). destruct (s[[e]](i)); reflexivity.
-    - subst. clear IHeval1.
+      generalize (HeqMu i). intro.
+      rewrite (elimT eqP (HeqMu i)). destruct (s[[e]](i)); reflexivity. }
+    { subst. clear IHeval1.
       inversion H0; subst.
-      rewrite fold_mask_of in *.
-      generalize (H (E_under_state s e) H6 s s' (conj H3 (fun i => refl_equal _))); intros.
+      move: (H (E_under_state s e) H6 s s' (conj H3 (fun i => refl_equal _))); intros.
       clear H HeqW.
-      assert (phi s') by (apply H1; rewrite <- meet_equiv, <- H2; assumption).
-      rewrite (meet_equiv m' (E_under_state s e)) in IHeval2.
-      generalize (IHeval2 (refl_equal _) H0 (fun i => e_and [m' i; s[[e]](i)]) (refl_equal _) H).
-      intros H4. clear IHeval2.
-      rewrite <- meet_equiv, H2 in H4.
-      generalize (E_While _ _ _ _ _ _ _ (refl_equal _) H1_ H1_0); intro H'.
-      unfold mask_of in H2, H1_.
-      rewrite H2 in H1_.
-      generalize (sub_meet _ _ (lem_2 _ _ H5 _ _ _ H1_)); intro.
-      rewrite fold_mask_of, (meet_comm _ (mask_of (E_under_state s' e))),
-      meet_assoc, <- (meet_assoc (mask_of m) (mask_of m)),
-      meet_double, meet_comm in H7.
-      rewrite H7, meet_comm in H4.
-      generalize (H4 (refl_equal _)); intro.
-      destruct H8.
-      split; try assumption.
-      generalize (lem_2_while _ _ H5 _ _ _ H'); intro.
-      intro.
-      generalize (H9 i) (H10 i); clear; intros.
-      unfold mask_of in *.
-      destruct (m' i); destruct (s[[e]](i)); destruct (s''[[e]](i));
-      try reflexivity;
-      try (inversion H; fail);
-      try (generalize (H0 (refl_equal _)); intro H'; inversion H').
+      rewrite 2!setI_e_and in IHeval2.
+      rewrite H2 in H1,H1_,IHeval2.
+      rewrite -setI_e_and in H1.
+      move: (IHeval2 erefl H0 (fun i => e_and [tuple m' i; s[[e]](i)]) erefl).       move: (elimT setIidPr (lem_2 _ _ H5 _ _ _ H1_)).
+      rewrite setICA -setIA setIA setIid setIA -?setI_e_and H2 => H4 H' {IHeval2}.
+      move: (H' H4 (H1 H1_)) => {H'} H7.
+      case:H7 => H7 H8.
+      split => // i {H7}.
+      move: (H8 i) => {H8}.
+      rewrite H2 in H1_0.
+      move: (elimT setIidPr (lem_2_while _ _ H5 _ _ _ (E_While _ _ _ _ _ _ _ erefl H1_ H1_0))).
+      rewrite /e_and/= int_of_boolK.
+      rewrite /mask_of.
+      move/setP => H8.
+      move: (H8 i) => {H8}.
+      rewrite 4!in_set.
+      move=> H7.
+      rewrite -andbA H7 //.
+    }
   Qed.
 
-  Theorem Soundness : forall phi (m : T -> Z) p psi,
+  Theorem Soundness : forall phi (m : T -> int) p psi,
                         Hoare_proof phi m p psi ->
                         regular p ->
                         hoare_quadruple phi m p psi.
   Proof.
     intros phi m p psi H.
     induction H; unfold hoare_quadruple in *; intros.
-    - inversion H1; subst; assumption.
-    - inversion H1; subst; simplify_mask;
-      unfold all in H0; unfold none in H0; apply H0.
-      + right. intro.
-        generalize (equal_f H4 i). unfold empty. intros H2.
-        destruct (m i); simpl in H2; try inversion H2; try reflexivity.
-      + left. intro.
-        generalize (equal_f H2 i). unfold T_mask. intros H3.
-        destruct (m i); simpl in H3; try inversion H3; try discriminate.
-    - apply H1. apply (IHHoare_proof H2 s); try apply H0; assumption.
-    - inversion H1; subst.
+    { inversion H1; subst; done. }
+    {
+      inversion H1; subst; apply H0.
+      { right => i.
+        apply setP in H4.
+        move: (H4 i).
+        rewrite /mask_of/empty in_set in_set0 /bool_of_int/negb.
+        case (m i == 0) => // . }
+      { left => i.
+        apply setP in H2.
+        move: (H2 i).
+        rewrite /mask_of/T_mask in_set in_setT // .
+      }
+    }
+    { apply H1.
+      apply (IHHoare_proof H2 s) => // .
+      apply H0 => // . }
+    { inversion H1; subst.
       inversion H3; subst;
       eapply (IHHoare_proof2 H7); try eapply (IHHoare_proof1 H6);
       try eassumption; rewrite <- H8; econstructor.
-    - destruct (lem_1 s s' n x es e m) as [H2 H2']. clear H2'.
+    }
+    {
+      destruct (lem_1 s s' n x es e m) as [H2 H2']. clear H2'.
       apply H2 in H1.
-      destruct H1 as [x0 [H1 H1']]; subst.
-      apply (H0 _ H1').
-    - inversion H3; inversion H5; subst.
-      + generalize (H0 _ H8 s' s' (conj H4 (fun i => refl_equal _))); intro.
-        rewrite <- meet_equiv, <- H13, meet_empty_l in H6.
-        generalize (H2 (E_under_state s' e) H10 s' s' (H6 (E_Inactive _ _))); intro.
-        rewrite <- meet_equiv, <- H13, meet_empty_l in H7.
-        apply (H7 (E_Inactive _ _ )).
-      + rewrite fold_mask_of, meet_equiv in H18.
-        rewrite fold_mask_of, diff_equiv in H19.
+      destruct H1 as [x0 [H1 H1']].
+      move: (H0 _ H1').
+        by rewrite H1.
+    }
+    {
+      inversion H3; inversion H5; subst.
+      { generalize (H0 _ H8 s' s' (conj H4 (fun i => refl_equal _))); intro.
+        rewrite -setI_e_and-H13/empty set0I in H6.
+        move: (H2 _ H10 s' s' (H6 (E_Inactive _ _))) => H7.
+        rewrite -setI_e_and-H13/empty set0I in H7.
+        apply (H7 (E_Inactive _ _ )). }
+      { rewrite setI_e_and in H18.
+        rewrite setD_e_and_neg in H19.
         apply (H2 (E_under_state s e) H10 s'0 s'
-                  (H0 _ H8 s s'0 (conj H4 (fun i => refl_equal _)) H18) H19).
-    - apply (Soundness_while _ _ _ _ H0 H1 _ _ m (refl_equal _) H3 H2).
+                  (H0 _ H8 s s'0 (conj H4 (fun i => refl_equal _)) H18) H19). }
+    }
+    { apply (Soundness_while _ _ _ _ H0 H1 _ _ m (refl_equal _) H3 H2). }
   Qed.
 
-  Definition wlp (m : T -> Z) P (phi : assertion) : assertion :=
+  Definition wlp (m : T -> int) P (phi : assertion) : assertion :=
     fun st => forall st', eval P (mask_of m) st st' ->
                           phi st'.
 
   Lemma while_sub :
     forall e p m s s' s'',
       stable e p ->
-      sub (meet m (mask_of (E_under_state s' e)))
-          (meet m (mask_of (E_under_state s e))) ->
-      eval (WHILE e DO p) (meet m (mask_of (E_under_state s' e))) s' s'' ->
-      eval (WHILE e DO p) (meet m (mask_of (E_under_state s e))) s' s''.
+      (m :&: mask_of (E_under_state s' e)) \subset (m :&: (mask_of (E_under_state s e))) ->
+      eval (WHILE e DO p) (m :&: (mask_of (E_under_state s' e))) s' s'' ->
+      eval (WHILE e DO p) (m :&: (mask_of (E_under_state s e))) s' s''.
   Proof.
     intros.
     generalize dependent s.
     remember (WHILE e DO p) as W.
-    remember (meet m (mask_of (E_under_state s' e))) as mu.
+    remember (m :&: (mask_of (E_under_state s' e))) as mu.
     induction H1; inversion HeqW; intros.
-    - eapply E_While; try eapply E_Inactive.
-      rewrite meet_assoc, (meet_comm (mask_of (E_under_state s0 e))),
-      fold_mask_of, <- meet_assoc, <- Heqmu, meet_empty_l.
-      reflexivity.
-    - subst.
-      generalize (sub_meet _ _ H1); intro.
-      generalize H0 H1_ H1_0; clear; intros.
-      rewrite (meet_comm m), meet_assoc, <- (meet_assoc m),
-      meet_double, <- meet_comm, <- (meet_comm m) in H0.
-      rewrite meet_assoc, meet_double in H1_, H1_0.
+    { eapply E_While; try eapply E_Inactive.
+      rewrite -setIA [mask_of _ :&: _]setIC setIA-Heqmu set0I // . }
+    { subst.
+      move: (elimT setIidPr H1) => H2.
+      rewrite setIA [_ :&: m]setIC setIA setIid in H2.
+      rewrite -setIA setIid in H1_,H1_0.
       econstructor.
-      + reflexivity.
-      + rewrite fold_mask_of; rewrite H0; eassumption.
-      + rewrite fold_mask_of; rewrite H0; eassumption.
+      { reflexivity. }
+      { rewrite H2; eassumption. }
+      { rewrite H2; eassumption. }
+    }
   Qed.
 
   Lemma H_Conseq_pre : forall (phi psi phi' : assertion) m p,
@@ -933,7 +907,16 @@ Section SIMT_Definition.
     apply (H_Conseq _ _ _ _ m p H H0 (fun s => id)).
   Qed.
 
-  Theorem Relative_Completeness' : forall phi (m : T -> Z) p psi,
+  Lemma H_Conseq_post : forall (phi psi psi' : assertion) m p,
+                         Hoare_proof phi m p psi' ->
+                         (forall s, psi' s -> psi s) ->
+                         Hoare_proof phi m p psi.
+  Proof.
+    intros.
+    apply (H_Conseq _ _ _ _ m p H (fun s => id) H0).
+  Qed.
+
+  Theorem Relative_Completeness' : forall phi (m : T -> int) p psi,
                                      regular p ->
                                      hoare_quadruple phi m p psi ->
                                      Hoare_proof (wlp m p psi) m p psi.
@@ -942,87 +925,87 @@ Section SIMT_Definition.
     generalize dependent m.
     generalize dependent phi.
     induction p; intros.
-    - rename t into es.
+    { rename t into es.
       eapply H_Conseq_pre.
-      + eapply H_Assign.
-      + simpl. intros.
+      { eapply H_Assign. }
+      { simpl. intros.
         eapply H1.
-        destruct v; apply lem_1; exists x'; split; try reflexivity; assumption.
-    - eapply H_Conseq_pre.
-      + econstructor.
-      + unfold wlp. intros. eapply H1. econstructor.
-    - unfold hoare_quadruple in H0.
+        destruct v; apply lem_1; exists x'; split; try reflexivity; assumption. }}
+    { eapply H_Conseq_pre.
+      { econstructor. }
+      { unfold wlp. intros. eapply H1. econstructor. }}
+    { unfold hoare_quadruple in H0.
       eapply H_Conseq_pre.
-      + econstructor.
-      + unfold wlp. intros. eapply H1.
+      { econstructor. }
+      { unfold wlp. intros. eapply H1.
         destruct H2;
           match goal with
             | [H2 : all m|-_] => apply lem_5_1 in H2
             | [H2 : none m|-_] => apply lem_5_2 in H2
-          end; try rewrite H2; try constructor.
-    - eapply H_Seq with (wlp m p2 psi).
-      + eapply H_Conseq_pre.
-        * inversion H; subst.
+          end; try rewrite H2; try constructor. }}
+    { eapply H_Seq with (wlp m p2 psi).
+      { eapply H_Conseq_pre.
+        { inversion H; subst.
           eapply IHp1; try assumption.
           unfold hoare_quadruple.
           unfold wlp. intros.
           unfold hoare_quadruple in H0.
           eapply H0 with (s:=s). eassumption.
-          econstructor; eassumption.
-        * intros. unfold wlp. intros.
+          econstructor; eassumption. }
+        { intros. unfold wlp. intros.
           eapply H1.
-          econstructor; eassumption.
-      + inversion H; subst.
+          econstructor; eassumption. }}
+      { inversion H; subst.
         eapply IHp2 with (wlp m p2 psi); try assumption.
         unfold hoare_quadruple, wlp. intros.
         eapply H1.
-        assumption.
-    - eapply H_If; intros.
-      + eapply H_Conseq_pre.
-        * inversion H; subst.
+        assumption. }}
+    { eapply H_If; intros.
+      { eapply H_Conseq_pre.
+        { inversion H; subst.
           eapply IHp1 with
           (phi :=
-             (fun s => wlp (fun i => e_and [m i; z i]) p1
-                           (wlp (fun i => e_and [m i; e_neg [z i]])
+             (fun s => wlp (fun i => e_and [tuple m i; z i]) p1
+                           (wlp (fun i => e_and [tuple m i; e_neg [tuple z i]])
                                 p2 psi) s /\
                        (forall i, s[[e]](i) = z i))); try assumption.
           unfold hoare_quadruple. intros.
           destruct H1.
           eapply H1.
-          eassumption.
-        * intros. destruct H1.
+          eassumption. }
+        { intros. destruct H1.
           unfold wlp. intros.
           unfold wlp in H1.
           apply H1.
-          rewrite <- meet_equiv in H3.
-          rewrite <- diff_equiv in H4.
-          econstructor;
-            try eapply H3; try eapply H4;
-            try (apply functional_extensionality; intro i;
-                 rewrite H2; reflexivity).
-      + inversion H; subst.
+          rewrite -setI_e_and in H3.
+          rewrite -setD_e_and_neg in H4.
+          econstructor; try eapply H3; try eapply H4.
+          apply setP => i.
+          rewrite /mask_of.
+          rewrite 2!in_set (H2 i) // . }}
+      { inversion H; subst.
         eapply IHp2 with
         (phi :=
-           (fun s => wlp (fun i => e_and [m i; e_neg [z i]]) p2 psi s /\
+           (fun s => wlp (fun i => e_and [tuple m i; e_neg [tuple z i]]) p2 psi s /\
                      (forall i, s[[e]](i) = z i))); try assumption.
         unfold hoare_quadruple. intros.
         destruct H1.
         unfold wlp in H1.
         eapply H1.
-        eassumption.
-    - inversion H; subst.
+        eassumption. }}
+    { inversion H; subst.
       remember
         (fun s =>
            exists z, (forall i, s[[e]](i) = z i) /\
-                     wlp (fun i => e_and [m i; z i]) (WHILE e DO p) psi s)
+                     wlp (fun i => e_and [tuple m i; z i]) (WHILE e DO p) psi s)
         as wp.
       assert (forall z,
                 Hoare_proof (fun s => wp s /\ (forall i, s[[e]](i) = z i))
-                            (fun i => e_and [m i; z i]) p wp).
-      + intros.
+                            (fun i => e_and [tuple m i; z i]) p wp).
+      { intros.
         unfold hoare_quadruple in H0.
         eapply H_Conseq_pre.
-        * eapply IHp with (phi:=fun s => wp s /\ (forall i, s[[e]](i) = z i));
+        { eapply IHp with (phi:=fun s => wp s /\ (forall i, s[[e]](i) = z i));
           try assumption; subst.
           unfold hoare_quadruple. intros.
           destruct H1 as [ [z' [H1 H1']] H1''].
@@ -1030,19 +1013,18 @@ Section SIMT_Definition.
           split; try reflexivity.
           unfold wlp. intros.
           apply H1'.
-          rewrite <- meet_equiv in H2, H5|-*.
+          rewrite -setI_e_and in H2, H5|-*.
           apply functional_extensionality in H1.
           apply functional_extensionality in H1''.
           rewrite <- H1.
           rewrite <- H1'' in H2.
           generalize H2 H3 H5; clear; intros.
-          econstructor.
-          reflexivity.
-          rewrite fold_mask_of, meet_assoc, meet_double; eassumption.
-          rewrite fold_mask_of, meet_assoc, meet_double.
+          econstructor; try rewrite -setI_e_and -setIA setIid => // ;
+            try eassumption.
           apply (lem_2 _ _ H3) in H2.
-          apply while_sub; assumption.
-        * intros.
+          rewrite -setI_e_and in H5.
+          apply while_sub; assumption. }
+        { intros.
           destruct H1.
           unfold wlp; intros.
           rewrite Heqwp in H1|-*.
@@ -1052,55 +1034,54 @@ Section SIMT_Definition.
           unfold wlp. intros.
           unfold wlp in H1'.
           apply H1'.
-          rewrite <- meet_equiv in H5, H6|-*.
+          rewrite -?setI_e_and in H5,H6|-*.
           apply functional_extensionality in H1.
           apply functional_extensionality in H2.
           rewrite <- H1.
           rewrite <- H2 in H5.
           generalize (lem_2 _ _ H3 _ _ _ H5); intro.
           econstructor; try apply while_sub; try eassumption.
-          rewrite fold_mask_of, meet_assoc, meet_double.
-          reflexivity.
-      + econstructor.
-        * eapply H_While. eassumption.
-        * intros.
+          rewrite -setIA setIid // . }}
+      { econstructor.
+        { eapply H_While. eassumption. }
+        { intros.
           rewrite Heqwp.
           exists (E_under_state s e).
           split; try reflexivity.
           unfold wlp. intros.
-          rewrite <- meet_equiv in H5.
+          rewrite -setI_e_and in H5.
           eapply H2.
           generalize H5; clear; intros.
-          rewrite meet_equiv in *.
+          rewrite setI_e_and in H5.
           remember (WHILE e DO p) as W.
-          remember (mask_of (fun i => e_and [m i; s[[e]](i)])) as mu.
+          remember (mask_of (fun i => e_and [tuple m i; s[[e]](i)])) as mu.
           induction H5; try (inversion HeqW).
           { eapply E_While; try eapply E_Inactive.
-            rewrite fold_mask_of, meet_equiv. rewrite <- Heqmu. reflexivity. }
+            rewrite setI_e_and -Heqmu // . }
           { subst.
             generalize H5_ H5_0; clear; intros.
-            unfold meet in *. rewrite <- meet_equiv in *.
-            rewrite fold_meet in *.
-            rewrite meet_assoc, meet_double in *.
+            rewrite -setI_e_and in H5_,H5_0.
             econstructor; try eassumption.
-            reflexivity. }
-        * cbv beta.
+            rewrite -setIA setIid // .
+          }}
+        { cbv beta.
           intros.
           destruct H2.
-          unfold none in H5.
+          apply lem_5_2 in H5.
           rewrite Heqwp in H2.
           destruct H2 as [z [H2 H2']].
           unfold wlp in H2'.
           eapply H2'.
-          assert (mask_of (fun i => e_and [m i; z i]) = empty) by
-              (apply functional_extensionality; intro i;
-               unfold mask_of;
-               rewrite <- (H2 i); rewrite (H5 i); reflexivity).
+          assert (mask_of (fun i => e_and [tuple m i; z i]) = empty).
+          { apply setP=> i.
+            apply setP in H5.
+            move: (H5 i).
+            rewrite ?in_set -(H2 i) => // . }
           rewrite H6.
-          econstructor.
+          econstructor. }}}
   Qed.
 
-  Theorem Relative_Completeness : forall phi (m : T -> Z) p psi,
+  Theorem Relative_Completeness : forall phi (m : T -> int) p psi,
                                     regular p ->
                                     hoare_quadruple phi m p psi ->
                                     Hoare_proof phi m p psi.
